Fixed admit in CertExecution2.v

src/traversal/TraversalConfigAltOld.v
@@ -81,106 +81,40 @@ Implicit Type WF : Wf G.
 Implicit Type WF_SC : wf_sc G sc.
 
 Record tc_coherent_alt_old :=
-  { tc_init : Init ∩₁ E ⊆₁ C ;
-    tc_C_in_E : C ⊆₁ E ;
-    tc_sb_C : dom_rel ( sb ⨾ ⦗C⦘) ⊆₁ C ;
-    tc_W_C_in_I : C ∩₁ W ⊆₁ I ;
-    tc_rf_C : dom_rel ( rf ⨾ ⦗C⦘) ⊆₁ I ;
-    tc_sc_C : dom_rel ( sc ⨾ ⦗C⦘) ⊆₁ C ;
-    tc_I_in_E : I ⊆₁ E ;
-    tc_I_in_W : I ⊆₁ W ;
-    tc_fwbob_I : dom_rel ( fwbob ⨾ ⦗I⦘) ⊆₁ C ;
-    tc_dr_pb_I : dom_rel ( (detour ∪ rfe) ⨾ (ppo ∪ bob) ⨾ ⦗I⦘) ⊆₁ I ;
-    tc_W_ex_sb_I : dom_rel (⦗W_ex_acq⦘ ⨾ sb ⨾ ⦗I⦘) ⊆₁ I
+  { otc_init : Init ∩₁ E ⊆₁ C ;
+    otc_C_in_E : C ⊆₁ E ;
+    otc_sb_C : dom_rel ( sb ⨾ ⦗C⦘) ⊆₁ C ;
+    otc_W_C_in_I : C ∩₁ W ⊆₁ I ;
+    otc_rf_C : dom_rel ( rf ⨾ ⦗C⦘) ⊆₁ I ;
+    otc_sc_C : dom_rel ( sc ⨾ ⦗C⦘) ⊆₁ C ;
+    otc_I_in_E : I ⊆₁ E ;
+    otc_I_in_W : I ⊆₁ W ;
+    otc_fwbob_I : dom_rel ( fwbob ⨾ ⦗I⦘) ⊆₁ C ;
+    otc_dr_pb_I : dom_rel ( (detour ∪ rfe) ⨾ (ppo ∪ bob) ⨾ ⦗I⦘) ⊆₁ I ;
+    otc_W_ex_sb_I : dom_rel (⦗W_ex_acq⦘ ⨾ sb ⨾ ⦗I⦘) ⊆₁ I
   }.
 
-(* move to imm_common.v *)
-Lemma bob_ppo_W_sb WF :
-  (bob ∪ ppo ∪ ⦗W_ex_acq⦘ ⨾ sb ⨾ ⦗W⦘)⁺ ⊆ ppo ∪ ppo ^? ;; (bob ∪ ⦗W_ex_acq⦘ ⨾ sb ⨾ ⦗W⦘)^+.
-Proof.
-arewrite (bob ∪ ppo ∪ ⦗W_ex_acq⦘ ⨾ sb ⨾ ⦗W⦘ ⊆
-         (bob ∪ ⦗W_ex_acq⦘ ⨾ sb ⨾ ⦗W⦘) ∪ ppo).
-basic_solver 12.
-apply ct_ind_left with (P:= fun r =>  r).
-by auto with hahn.
-- arewrite(bob ⊆ (bob ∪ ⦗W_ex_acq⦘ ⨾ sb ⨾ ⦗W⦘)⁺).
-  arewrite(⦗W_ex_acq⦘ ⨾ sb ⨾ ⦗W⦘ ⊆ (bob ∪ ⦗W_ex_acq⦘ ⨾ sb ⨾ ⦗W⦘)⁺) at 2.
-  basic_solver 12.
-- intros k H. rewrite H; clear k H; rewrite crE; relsf; unionL.
-+ rewrite (bob_ppo WF). 
-  arewrite(bob ⊆ (bob ∪ ⦗W_ex_acq⦘ ⨾ sb ⨾ ⦗W⦘)⁺).
-  basic_solver.
-+ rewrite (wf_ppoD) at 1. type_solver.
-+ rewrite (wf_ppoD) at 1 2. type_solver.
-+ arewrite(bob ⊆ (bob ∪ ⦗W_ex_acq⦘ ⨾ sb ⨾ ⦗W⦘)^*); relsf.
-+ sin_rewrite (bob_ppo WF). 
-  arewrite(bob ⊆ (bob ∪ ⦗W_ex_acq⦘ ⨾ sb ⨾ ⦗W⦘)^*); relsf.
-+ arewrite(⦗W_ex_acq⦘ ⨾ sb ⨾ ⦗W⦘ ⊆ (bob ∪ ⦗W_ex_acq⦘ ⨾ sb ⨾ ⦗W⦘)^*) at 1; relsf.
-+ rewrite (wf_ppoD) at 1. type_solver.
-+ basic_solver 12.
-+ rewrite (wf_ppoD) at 1 2. type_solver.
-Qed.
-
-(* move to imm_common.v *)
-Lemma bob_sb :
-  (bob ∪ ⦗W_ex_acq⦘ ⨾ sb ⨾ ⦗W⦘)^+ ⨾ ⦗W⦘ ⊆ 
-  bob^+ ⨾ (⦗W_ex_acq⦘ ⨾ sb ⨾ ⦗W⦘)^? ⨾ ⦗W⦘ ∪ ⦗W_ex_acq⦘ ⨾ sb ⨾ ⦗W⦘.
-Proof.
-apply ct_ind_left with (P:= fun r =>  r ⨾ ⦗W⦘).
-by auto with hahn.
-by arewrite (bob ⊆ bob⁺); basic_solver 12.
-intros k H.
-rewrite !seqA; rewrite H; clear k H.
-relsf; unionL.
-- arewrite(bob ⊆ bob^*) at 1; relsf.
-- sin_rewrite bob_in_sb.
-generalize (@sb_trans G); ins; relsf.
-basic_solver 12.
-- arewrite (bob ⊆ bob⁺); basic_solver 12.
-- generalize (@sb_trans G); basic_solver 12.
-Qed.
-
-(* move to imm_common.v *)
-Lemma tc_bob :
-  bob^+ ⊆ fwbob^+ ∪ ⦗R ∩₁ Acq⦘ ⨾ sb.
-Proof.
-unfold imm_common.bob.
-apply ct_ind_left with (P:= fun r =>  r).
-by auto with hahn.
-by arewrite (fwbob ⊆ fwbob⁺); basic_solver 12.
-intros k H.
-rewrite H; clear k H.
-relsf; unionL.
-- by arewrite (fwbob ⊆ fwbob^*); relsf; basic_solver 12.
-- sin_rewrite (fwbob_in_sb).
-  generalize (@sb_trans G); ins; relsf; basic_solver 12.
-- arewrite (⦗R ∩₁ Acq⦘ ⊆ ⦗R⦘). basic_solver.
-  sin_rewrite fwbob_r_sb.
-  by arewrite (fwbob ⊆ fwbob^+); basic_solver 21.
-- generalize (@sb_trans G); basic_solver 12.
-Qed.
-
-Lemma tc_tc_fwbob_I (tc_old : tc_coherent_alt_old) :
+Lemma otc_tc_fwbob_I (tc_old : tc_coherent_alt_old) :
   dom_rel (fwbob⁺ ⨾ ⦗I⦘) ⊆₁ C.
 Proof.
 rewrite ct_end, !seqA.
-rewrite (dom_rel_helper (tc_fwbob_I tc_old)).
+rewrite (dom_rel_helper (otc_fwbob_I tc_old)).
 rewrite fwbob_in_sb.
 generalize (@sb_trans G); ins; relsf.
-generalize (tc_sb_C tc_old).
+generalize (otc_sb_C tc_old).
 basic_solver 12.
 Qed.
 
-Lemma tc_W_bob_I (tc_old : tc_coherent_alt_old) :
+Lemma otc_W_bob_I (tc_old : tc_coherent_alt_old) :
   dom_rel (⦗W⦘ ⨾ bob⁺ ⨾ ⦗I⦘) ⊆₁ I.
 Proof.
 rewrite tc_bob; relsf; splits; [| type_solver].
-rewrite (dom_rel_helper (tc_tc_fwbob_I tc_old)).
-generalize (tc_W_C_in_I tc_old).
+rewrite (dom_rel_helper (otc_tc_fwbob_I tc_old)).
+generalize (otc_W_C_in_I tc_old).
 basic_solver 12.
 Qed.
 
-Lemma tc_I_ar_I_implied_helper_1 WF (tc_old : tc_coherent_alt_old) :
+Lemma otc_I_ar_I_implied_helper_1 WF (tc_old : tc_coherent_alt_old) :
   dom_rel (⦗W⦘ ⨾  (bob ∪ ppo ∪ ⦗W_ex_acq⦘ ⨾ sb ⨾ ⦗W⦘)^+ ⨾ ⦗I⦘) ⊆₁ I.
 Proof.
 rewrite (bob_ppo_W_sb WF).
@@ -188,17 +122,17 @@ rewrite crE.
 rewrite wf_ppoD at 1 2.
 relsf; splits; try type_solver.
 arewrite (⦗I⦘ ⊆ ⦗W⦘ ;; ⦗I⦘).
-by generalize (tc_I_in_W tc_old); basic_solver.
+by generalize (otc_I_in_W tc_old); basic_solver.
 sin_rewrite bob_sb; relsf; splits.
 + rewrite !seqA.
   arewrite ((⦗W_ex_acq⦘ ⨾ sb ⨾ ⦗W⦘)^? ⨾ ⦗W⦘ ⨾ ⦗I⦘ ⊆ ⦗I⦘ ⨾ sb^?).
-  by generalize (tc_W_ex_sb_I tc_old); basic_solver 12.
-  generalize (tc_W_bob_I tc_old); basic_solver 12.
-+ generalize (tc_W_ex_sb_I tc_old).
+  by generalize (otc_W_ex_sb_I tc_old); basic_solver 12.
+  generalize (otc_W_bob_I tc_old); basic_solver 12.
++ generalize (otc_W_ex_sb_I tc_old).
   basic_solver 12.
 Qed.
 
-Lemma tc_I_ar_I_implied_helper_2  WF WF_SC (tc_old : tc_coherent_alt_old) :
+Lemma otc_I_ar_I_implied_helper_2  WF WF_SC (tc_old : tc_coherent_alt_old) :
    dom_rel (<|W|> ;; ar⁺ ;; <|I|>) ⊆₁ I.
 Proof.
   unfold imm_s.ar, ar_int.
@@ -212,11 +146,11 @@ Proof.
   arewrite (srd ∪ srd ⨾ bps⁺ ⊆ srd ⨾ bps^*).
   by rewrite rtE; basic_solver 12.
   relsf; splits.
-- generalize (tc_I_ar_I_implied_helper_1 WF tc_old).
+- generalize (otc_I_ar_I_implied_helper_1 WF tc_old).
   rewrite <- Heqbps; basic_solver 21.
 - rewrite !seqA, <- dom_eqv1.
   arewrite (⦗W⦘ ⨾ bps＊ ⨾ (srd ⨾ bps＊)⁺ ⨾ ⦗I⦘ ⊆ ⦗I⦘ ⨾ (fun _ _ => True)); cycle 1.
-  by generalize (tc_W_C_in_I tc_old); basic_solver.
+  by generalize (otc_W_C_in_I tc_old); basic_solver.
   rewrite inclusion_t_rt.
   arewrite (I ⊆₁ I ∪₁ C ∩₁ F ∩₁ Sc) at 1.
   apply rt_ind_right with (P:= fun r =>  ⦗W⦘ ⨾ bps＊ ⨾ r ⨾ ⦗I ∪₁ C ∩₁ F ∩₁ Sc⦘).
@@ -227,7 +161,7 @@ subst.
 unionL.
 type_solver.
 rewrite id_union; relsf; unionL.
-* rewrite (dom_rel_helper (tc_I_ar_I_implied_helper_1 WF tc_old)); subst.
+* rewrite (dom_rel_helper (otc_I_ar_I_implied_helper_1 WF tc_old)); subst.
 basic_solver 12.
 *
 rewrite (ppo_in_sb WF), bob_in_sb.
@@ -236,21 +170,21 @@ arewrite_id ⦗W⦘ at 2.
 generalize (@sb_trans G); ins; relsf.
 arewrite (⦗C ∩₁ F ∩₁ Sc⦘ ⊆  ⦗C⦘).
 basic_solver.
-rewrite (dom_rel_helper (tc_sb_C tc_old)).
-generalize (tc_W_C_in_I tc_old); basic_solver.
+rewrite (dom_rel_helper (otc_sb_C tc_old)).
+generalize (otc_W_C_in_I tc_old); basic_solver.
 + intros k H; rewrite !seqA.
 rewrite rtE at 2; relsf; unionL; subst srd.
 
 *
 rewrite (wf_scD WF_SC).
-rewrite (tc_I_in_W tc_old) at 1.
+rewrite (otc_I_in_W tc_old) at 1.
 rewrite (dom_r (wf_rfeD WF)).
 rewrite (dom_r (wf_detourD WF)).
 rewrite id_union; relsf; unionL; try type_solver.
 
 rewrite !seqA.
 arewrite (⦗F ∩₁ Sc⦘ ⨾ sc ⨾ ⦗F ∩₁ Sc⦘ ⨾ ⦗C ∩₁ F ∩₁ Sc⦘ ⊆ ⦗I ∪₁ C ∩₁ F ∩₁ Sc⦘ ⨾ (fun _ _ : actid => True)).
-generalize (tc_sc_C tc_old); basic_solver 21.
+generalize (otc_sc_C tc_old); basic_solver 21.
 sin_rewrite H; basic_solver.
 
 
@@ -271,10 +205,10 @@ rewrite id_union; relsf; unionL.
 ++ 
 arewrite (⦗F ∩₁ Sc⦘ ⨾ sb ⊆  fwbob).
 by unfold imm_common.fwbob; mode_solver.
-generalize (tc_sc_C tc_old) (tc_fwbob_I tc_old).
+generalize (otc_sc_C tc_old) (otc_fwbob_I tc_old).
 basic_solver 21.
 ++ 
-generalize (tc_sc_C tc_old) (tc_sb_C tc_old).
+generalize (otc_sc_C tc_old) (otc_sb_C tc_old).
 basic_solver 21.
 
 -- cut (rd ⨾ bps^+ ⨾ ⦗I ∪₁ C ∩₁ F ∩₁ Sc⦘ ⊆ ⦗I⦘ ;; (fun _ _ : actid => True)).
@@ -282,27 +216,27 @@ by intro A; sin_rewrite A; arewrite (I ⊆₁ I ∪₁ C ∩₁ F ∩₁ Sc) at 
 subst bps.
 rewrite (bob_ppo_W_sb WF); relsf; unionL.
 rewrite id_union; relsf; unionL.
-by generalize (tc_dr_pb_I tc_old); subst rd; basic_solver 12.
+by generalize (otc_dr_pb_I tc_old); subst rd; basic_solver 12.
 by rewrite wf_ppoD; type_solver.
 rewrite id_union; relsf; unionL.
 ++ arewrite (⦗I⦘ ⊆ ⦗W⦘ ;; ⦗I⦘).
-by generalize (tc_I_in_W tc_old); basic_solver.
+by generalize (otc_I_in_W tc_old); basic_solver.
 sin_rewrite bob_sb; relsf; unionL.
 ** rewrite !seqA.
 arewrite ((⦗W_ex_acq⦘ ⨾ sb ⨾ ⦗W⦘)^? ⨾ ⦗W⦘ ⨾ ⦗I⦘ ⊆ ⦗I⦘ ⨾ (fun _ _ : actid => True)).
-by generalize (tc_W_ex_sb_I tc_old); basic_solver 21.
+by generalize (otc_W_ex_sb_I tc_old); basic_solver 21.
 rewrite crE; relsf; unionL.
 --- rewrite tc_bob; relsf; unionL.
-2: by generalize (tc_dr_pb_I tc_old); subst rd; unfold imm_common.bob; basic_solver 21.
-seq_rewrite (dom_rel_helper (tc_tc_fwbob_I  tc_old)).
+2: by generalize (otc_dr_pb_I tc_old); subst rd; unfold imm_common.bob; basic_solver 21.
+seq_rewrite (dom_rel_helper (otc_tc_fwbob_I  tc_old)).
 subst rd; relsf; unionL.
-generalize (tc_rf_C tc_old); unfold Execution.rfe; basic_solver 21.
+generalize (otc_rf_C tc_old); unfold Execution.rfe; basic_solver 21.
 rewrite (dom_l (wf_detourD WF)).
 rewrite detour_in_sb.
-generalize (tc_sb_C tc_old) (tc_W_C_in_I tc_old); basic_solver 21.
+generalize (otc_sb_C tc_old) (otc_W_C_in_I tc_old); basic_solver 21.
 --- rewrite wf_ppoD, !seqA.
-seq_rewrite (dom_rel_helper (tc_W_bob_I tc_old)).
-generalize (tc_dr_pb_I tc_old).
+seq_rewrite (dom_rel_helper (otc_W_bob_I tc_old)).
+generalize (otc_dr_pb_I tc_old).
 subst rd.
 basic_solver 21.
 ** 
@@ -313,7 +247,7 @@ rewrite (dom_r (wf_detourD WF)).
 rewrite (W_ex_in_W WF).
 type_solver.
 ---
-generalize (tc_dr_pb_I tc_old) (tc_W_ex_sb_I tc_old).
+generalize (otc_dr_pb_I tc_old) (otc_W_ex_sb_I tc_old).
 basic_solver 21.
 ++ rewrite (ppo_in_sb WF), bob_in_sb.
 arewrite_id ⦗W_ex_acq⦘.
@@ -321,12 +255,12 @@ arewrite_id ⦗W⦘.
 generalize (@sb_trans G); ins; relsf.
 arewrite (⦗C ∩₁ F ∩₁ Sc⦘ ⊆  ⦗C⦘).
 basic_solver.
-rewrite (dom_rel_helper (tc_sb_C tc_old)).
+rewrite (dom_rel_helper (otc_sb_C tc_old)).
 subst rd; relsf; unionL.
-generalize (tc_rf_C tc_old); unfold Execution.rfe; basic_solver 21.
+generalize (otc_rf_C tc_old); unfold Execution.rfe; basic_solver 21.
 rewrite (dom_l (wf_detourD WF)).
 rewrite detour_in_sb.
-generalize (tc_sb_C tc_old) (tc_W_C_in_I tc_old); basic_solver 21.
+generalize (otc_sb_C tc_old) (otc_W_C_in_I tc_old); basic_solver 21.
 
 Qed.
 
